ROOT
@@ -1,5 +1,7 @@
 session "Interaction_Trees" = "Shallow-Expressions-Z" +
   options [timeout = 600, document = pdf, document_output = "output"]
+  sessions
+    Abstract_Prog_Syntax
   theories
     ITrees
   document_files
